fixed last two lemmas

coq/Shifting.v
@@ -1,4 +1,5 @@
 (** * Shifting in System FC *)
+Require Import Omega.
 Require Export SystemFC.
 
 Module SHIFTING.
@@ -7,14 +8,27 @@ Import SYSTEMFC.
 (* ################################### *)
 (** *** Types *)
 
+Class ShiftTyp (X : Type) := {
+  shift_typ : nat -> X -> X                                     
+}.
+
+Class ShiftCoercion (X : Type) := {
+  shift_cn : nat -> X -> X                                     
+}.
+
+
 (* Types in Types *)
 Fixpoint tshift (X : nat) (T : ty) : ty :=
   match T with
-  | TVar Y          => TVar (if le_gt_dec X Y then 1 + Y else Y)
-  | TArrow T1 T2    => TArrow (tshift X T1) (tshift X T2)
-  | TUniv T2        => TUniv (tshift (1 + X) T2)
-  | TCoerce T1 T2 T => TCoerce (tshift X T1) (tshift X T2) (tshift X T) 
+    | TVar Y          => TVar (if le_gt_dec X Y then 1 + Y else Y)
+    | TCon Y        => TCon Y
+    | TApp T1 T2    => TApp (tshift X T1) (tshift X T2)
+    | TUniv K T2        => TUniv K (tshift (1 + X) T2)
   end.
+
+Instance shift_type_type : ShiftTyp ty := {
+   shift_typ := tshift
+}.                                                      
 
 (* ################################### *)
 (** *** Coercions *)
@@ -26,10 +40,9 @@ Fixpoint cshift (X : nat) (c : cn) : cn :=
   | CRefl T           => CRefl T
   | CSym c            => CSym (cshift X c)
   | CTrans c1 c2      => CTrans (cshift X c1) (cshift X c2)
-  | CArrow c1 c2      => CArrow (cshift X c1) (cshift X c2)
-  | CTCoerce c1 c2 c3 => CTCoerce (cshift X c1) (cshift X c2) (cshift X c3)
+  | CApp c1 c2      => CApp (cshift X c1) (cshift X c2)
   | CNth n c          => CNth n (cshift X c)
-  | CTAbs c           => CTAbs (cshift X c)
+  | CTAbs k c           => CTAbs k (cshift X c)
   | CTApp c T         => CTApp (cshift X c) T
   end.
 
@@ -40,13 +53,19 @@ Fixpoint cshift_typ (X : nat) (c : cn) : cn :=
   | CRefl T           => CRefl (tshift X T)
   | CSym c            => CSym (cshift_typ X c)
   | CTrans c1 c2      => CTrans (cshift_typ X c1) (cshift_typ X c2)
-  | CArrow c1 c2      => CArrow (cshift_typ X c1) (cshift_typ X c2)
-  | CTCoerce c1 c2 c3 => CTCoerce (cshift_typ X c1) (cshift_typ X c2)
-                                  (cshift_typ X c3)
+  | CApp c1 c2      => CApp (cshift_typ X c1) (cshift_typ X c2)
   | CNth n c          => CNth n (cshift_typ X c)
-  | CTAbs c           => CTAbs (cshift_typ (S X) c)
+  | CTAbs k c           => CTAbs k (cshift_typ (S X) c)
   | CTApp c T         => CTApp (cshift_typ X c) (tshift X T)
   end.
+
+Instance shift_cn_cn : ShiftCoercion cn := {
+  shift_cn := cshift
+}.                      
+Instance shift_typ_cn : ShiftTyp cn := {
+   shift_typ := cshift_typ
+}.                                                      
+
 
 (* ################################### *)
 (** *** Terms *)
@@ -57,7 +76,7 @@ Fixpoint shift (x:nat) (t:tm) : tm :=
     | tvar y         => tvar (if le_gt_dec x y then S y else y)
     | tabs T1 t2     => tabs T1 (shift (S x) t2)
     | tapp t1 t2     => tapp (shift x t1) (shift x t2)
-    | ttabs t2       => ttabs (shift x t2)
+    | ttabs k t2       => ttabs k (shift x t2)
     | ttapp t1 T2    => ttapp (shift x t1) T2
     | tcapp t1 c2    => tcapp (shift x t1) c2
     | tcabs T1 T2 t2 => tcabs T1 T2 (shift x t2)
@@ -65,29 +84,37 @@ Fixpoint shift (x:nat) (t:tm) : tm :=
   end.
 
 (* Coercions in Terms *)
-Fixpoint shift_cn (X : nat) (t : tm) : tm :=
+Fixpoint tshift_cn (X : nat) (t : tm) : tm :=
   match t with
     | tvar y         => tvar y
-    | tabs T1 t2     => tabs T1 (shift_cn X t2)
-    | tapp t1 t2     => tapp (shift_cn X t1) (shift_cn X t2)
-    | ttabs t2       => ttabs (shift_cn X t2)
-    | ttapp t1 T2    => ttapp (shift_cn X t1) T2
-    | tcapp t1 c2    => tcapp (shift_cn X t1) (cshift X c2)
-    | tcabs T1 T2 t2 => tcabs T1 T2 (shift_cn (S X) t2)
-    | tcoerce t c    => tcoerce (shift_cn X t) (cshift X c)
+    | tabs T1 t2     => tabs T1 (tshift_cn X t2)
+    | tapp t1 t2     => tapp (tshift_cn X t1) (tshift_cn X t2)
+    | ttabs k t2       => ttabs k (tshift_cn X t2)
+    | ttapp t1 T2    => ttapp (tshift_cn X t1) T2
+    | tcapp t1 c2    => tcapp (tshift_cn X t1) (cshift X c2)
+    | tcabs T1 T2 t2 => tcabs T1 T2 (tshift_cn (S X) t2)
+    | tcoerce t c    => tcoerce (tshift_cn X t) (cshift X c)
   end.
 
 (* Types in Terms *)
-Fixpoint shift_typ (X : nat) (t : tm) {struct t} : tm :=
+Fixpoint tshift_typ (X : nat) (t : tm) {struct t} : tm :=
   match t with
     | tvar y         => tvar y
-    | tabs T1 t2     => tabs (tshift X T1) (shift_typ X t2)
-    | tapp t1 t2     => tapp (shift_typ X t1) (shift_typ X t2)
-    | ttabs t2       => ttabs (shift_typ (1 + X) t2)
-    | ttapp t1 T2    => ttapp (shift_typ X t1) (tshift X T2)
-    | tcapp t1 c2    => tcapp (shift_typ X t1) (cshift_typ X c2)
-    | tcabs T1 T2 t2 => tcabs (tshift X T1) (tshift X T2) (shift_typ X t2)
-    | tcoerce t1 c2  => tcoerce (shift_typ X t1) (cshift_typ X c2)
+    | tabs T1 t2     => tabs (tshift X T1) (tshift_typ X t2)
+    | tapp t1 t2     => tapp (tshift_typ X t1) (tshift_typ X t2)
+    | ttabs k t2       => ttabs k (tshift_typ (1 + X) t2)
+    | ttapp t1 T2    => ttapp (tshift_typ X t1) (tshift X T2)
+    | tcapp t1 c2    => tcapp (tshift_typ X t1) (cshift_typ X c2)
+    | tcabs T1 T2 t2 => tcabs (tshift X T1) (tshift X T2) (tshift_typ X t2)
+    | tcoerce t1 c2  => tcoerce (tshift_typ X t1) (cshift_typ X c2)
   end.
+
+
+Instance shift_cn_tm : ShiftCoercion tm := {
+  shift_cn := tshift_cn
+}.                      
+Instance shift_typ_tm : ShiftTyp tm := {
+   shift_typ := tshift_typ
+}.                                                      
 
 End SHIFTING.
