coq/SystemFC.v
@@ -1,5 +1,5 @@
-(** * System FC **)
 
+(** * System FC **)
 Require Export SfLib.
 
 
@@ -11,11 +11,21 @@ Module SYSTEMFC.
 (* ################################### *)
 (** *** Types *)
 
+Inductive kind : Type :=
+ | KStar : kind
+ | KArrow : kind -> kind -> kind.
+  
+Inductive tycon : Type :=
+| TArrow  : tycon
+| TEq     : kind -> tycon
+| TData   : nat -> tycon.
+  
 Inductive ty : Type := 
-  | TVar    : nat -> ty 
-  | TArrow  : ty -> ty -> ty
-  | TUniv   : ty -> ty
-  | TCoerce : ty -> ty -> ty -> ty.
+| TVar   : nat -> ty
+| TCon   : tycon -> ty
+| TApp   : ty -> ty -> ty
+| TUniv  : kind -> ty -> ty.
+
 
 (* ################################### *)
 (** *** Coercions *)
@@ -25,17 +35,16 @@ Inductive cn : Type :=
   | CRefl    : ty -> cn
   | CSym     : cn -> cn
   | CTrans   : cn -> cn -> cn
-  | CArrow   : cn -> cn -> cn
-  | CTCoerce : cn -> cn -> cn -> cn
+  | CApp     : cn -> cn -> cn
   | CNth     : nat -> cn -> cn
-  | CTAbs    : cn -> cn
+  | CTAbs    : kind -> cn -> cn
   | CTApp    : cn -> ty -> cn.
 
 Tactic Notation "c_cases" tactic(first) ident(c) :=
   first;
   [ Case_aux c "CVar"   | Case_aux c "CRefl"
   | Case_aux c "CSym"   | Case_aux c "CTrans"
-  | Case_aux c "CArrow" | Case_aux c "CTCoerce"
+  | Case_aux c "CApp"  (* | Case_aux c "CTCoerce" *)
   | Case_aux c "CNth"
   | Case_aux c "CTAbs"  | Case_aux c "CTApp" ].
 
@@ -48,7 +57,7 @@ Inductive tm : Type :=
   | tapp    : tm -> tm -> tm
   | tabs    : ty -> tm -> tm
   | ttapp   : tm -> ty -> tm
-  | ttabs   : tm -> tm
+  | ttabs   : kind -> tm -> tm
   | tcapp   : tm -> cn -> tm
   | tcabs   : ty -> ty -> tm -> tm
   | tcoerce : tm -> cn -> tm.
@@ -67,8 +76,8 @@ Tactic Notation "t_cases" tactic(first) ident(c) :=
 Inductive uncoerced_value : tm -> Prop :=
   | uv_abs : forall T t,
       uncoerced_value (tabs T t)
-  | uv_tabs : forall t,
-      uncoerced_value (ttabs t)
+  | uv_tabs : forall t k,
+      uncoerced_value (ttabs k t)
   | uv_cabs : forall t T1 T2,
       uncoerced_value (tcabs T1 T2 t).
 
