coq/Typing.v
@@ -1,3 +1,4 @@
+Require Import SystemFC.
 Require Export Shifting.
 Require Export Substitution.
 
@@ -12,10 +13,16 @@ Import SUBSTITUTION.
 (* ################################### *)
 (** *** Contexts *)
 
+Parameter Sigma : tycon -> option kind.
+
+Axiom arrKind : Sigma TArrow = Some (KArrow KStar (KArrow KStar KStar)).
+Axiom coerceKind : forall k,
+   Sigma (TEq k) = Some (KArrow k (KArrow k (KArrow KStar KStar))).
+
 Inductive context : Set :=
   | empty    : context
   | ext_var  : context -> ty -> context
-  | ext_tvar : context -> context
+  | ext_tvar : context -> kind -> context
   | ext_cvar : context -> ty * ty -> context.
 
 Definition opt_map {A B : Type} (f : A -> B) (x : option A) :=
@@ -38,17 +45,17 @@ Fixpoint get_var (E : context) (x : nat) : option ty :=
         | O   => Some T
         | S y => get_var E' y
       end
-    | ext_tvar E'   => opt_map (tshift 0) (get_var E' x)
+    | ext_tvar E' k => opt_map (tshift 0) (get_var E' x)
     | ext_cvar E' _ => get_var E' x
   end.
 
-Fixpoint get_tvar (E : context) (N : nat) : bool :=
+Fixpoint get_tvar (E : context) (N : nat) : option kind :=
   match E with
-    | empty => false
+    | empty =>  None
     | ext_var E' _ => get_tvar E' N
-    | ext_tvar E'  =>
+    | ext_tvar E' k  =>
       match N with
-        | O => true
+        | O => Some k
         | S N' => get_tvar E' N'
       end
     | ext_cvar E' _ => get_tvar E' N
@@ -58,7 +65,7 @@ Fixpoint get_cvar (E : context) (N : nat) : option (ty * ty) :=
   match E with
     | empty => None
     | ext_var E' _  => get_cvar E' N
-    | ext_tvar E'   => opt_map_prod (tshift 0) (get_cvar E' N)
+    | ext_tvar E' _  => opt_map_prod (tshift 0) (get_cvar E' N)
     | ext_cvar E' c =>
       match N with
         | O    => Some c
@@ -70,45 +77,47 @@ Fixpoint get_cvar (E : context) (N : nat) : option (ty * ty) :=
 (* ################################### *)
 (** *** Well Formed Types *)
 
-Fixpoint wf_ty (Gamma : context) (T : ty) : Prop :=
+Fixpoint wf_ty (Gamma : context) (T : ty) (k : kind) : Prop :=
   match T with
-  | TVar X          => get_tvar Gamma X = true
-  | TArrow T1 T2    => wf_ty Gamma T1 /\ wf_ty Gamma T2
-  | TUniv  T        => wf_ty (ext_tvar Gamma) T
-  | TCoerce T1 T2 T => wf_ty Gamma T1 /\ wf_ty Gamma T2 /\ wf_ty Gamma T
+    | TVar X        => get_tvar Gamma X = Some k
+    | TCon tc       => Sigma tc = Some k
+    | TApp T1 T2    => exists k', wf_ty Gamma T1 (KArrow k' k) /\ wf_ty Gamma T2 k'
+    | TUniv k' T    => k = KStar /\ wf_ty (ext_tvar Gamma k') T KStar
+
   end.
 
-Inductive well_formed_type (Gamma : context) : ty -> Prop :=
-  | WF_TVar : forall X,
-      get_tvar Gamma X = true ->
-      well_formed_type Gamma (TVar X)
-  | WF_TArrow : forall T1 T2,
-      well_formed_type Gamma T1 ->
-      well_formed_type Gamma T2 ->
-      well_formed_type Gamma (TArrow T1 T2)
-  | WF_TUniv : forall T,
-      well_formed_type (ext_tvar Gamma) T ->
-      well_formed_type Gamma (TUniv T)
-  | WF_TCoerce : forall T T1 T2,
-      well_formed_type Gamma T1 ->
-      well_formed_type Gamma T2 ->
-      well_formed_type Gamma T  ->
-      well_formed_type Gamma (TCoerce T1 T2 T).
+Inductive well_formed_type (Gamma : context) : ty -> kind -> Prop :=
+  | WF_TVar : forall X k,
+      get_tvar Gamma X = Some k ->
+      well_formed_type Gamma (TVar X) k
+  | WF_TCon : forall X k,
+      Sigma X = Some k ->
+      well_formed_type Gamma (TCon X) k
+  | WF_TApp : forall T1 T2 k' k,
+      well_formed_type Gamma T1 (KArrow k' k) ->
+      well_formed_type Gamma T2 k' ->
+      well_formed_type Gamma (TApp T1 T2) k
+  | WF_TUniv : forall k T,
+      well_formed_type (ext_tvar Gamma k) T KStar ->
+      well_formed_type Gamma (TUniv k T) KStar.
 
-Lemma wf_type_correct : forall Gamma T,
-  well_formed_type Gamma T <-> wf_ty Gamma T.
+Lemma wf_type_correct : forall Gamma T k,
+  well_formed_type Gamma T k <-> wf_ty Gamma T k.
 Proof.
+
   split; intros.
   Case "->".
     induction H; try split; try split; trivial.
+    exists k'. split; trivial.
   Case "<-".
-    generalize dependent Gamma. induction T.
+    generalize dependent Gamma. generalize dependent k. induction T; intros k' Gamma H.
     constructor. simpl in H. trivial.
-    constructor; simpl in H; inversion H. apply IHT1. trivial.
+    constructor. simpl in H. trivial.
+    inversion H. destruct H0.
+    apply WF_TApp with (k' := x). apply IHT1. trivial.
       apply IHT2. trivial.
-    constructor. simpl in H. apply IHT. trivial.
-    constructor; simpl in H; inversion H; inversion H1. apply IHT1. trivial.
-      apply IHT2. trivial. apply IHT3. trivial.
+    inversion H. subst.
+      constructor. simpl in H. apply IHT. trivial.
 Qed.
 
 
@@ -120,105 +129,80 @@ Inductive well_formed_context : context -> Prop :=
   | WFC_empty :
       well_formed_context empty
   | WFC_ext_var : forall T Gamma,
-      well_formed_type Gamma T ->
+      well_formed_type Gamma T KStar ->
       well_formed_context Gamma ->
-      well_formed_context (ext_var Gamma T)
-  | WFC_ext_tvar : forall Gamma,
+      well_formed_context (ext_var Gamma T) 
+  | WFC_ext_tvar : forall Gamma k,
       well_formed_context Gamma ->
-      well_formed_context (ext_tvar Gamma)
-  | WFC_ext_cvar : forall Gamma U V,
+      well_formed_context (ext_tvar Gamma k)
+  | WFC_ext_cvar : forall Gamma U V k,
       well_formed_context Gamma ->
-      well_formed_type Gamma U  ->
-      well_formed_type Gamma V  ->
+      well_formed_type Gamma U k ->
+      well_formed_type Gamma V k ->
       well_formed_context (ext_cvar Gamma (U, V)).
 
-
-Inductive subst_context : ty -> nat -> context -> context -> Prop := 
-  | s_ext_var : forall T n Gamma Gamma' U U',
-      subst_context T n Gamma Gamma' ->
-      subst_type_in_type T n U U' ->
-      subst_context T n (ext_var Gamma U) (ext_var Gamma' U')
-  | s_ext_tvar0 : forall T Gamma,
-      (* the variable is removed because it has been replaced *)
-      well_formed_type Gamma T  ->
-      well_formed_context Gamma ->
-      subst_context T 0 (ext_tvar Gamma) Gamma
-  | s_ext_tvar : forall T n Gamma Gamma',
-      subst_context T n Gamma Gamma' ->
-      subst_context (tshift 0 T) (S n) (ext_tvar Gamma) (ext_tvar Gamma')
-  | s_ext_cvar : forall T U1 V1 U2 V2 n Gamma Gamma',
-      subst_context T n Gamma Gamma' ->
-      subst_type_in_type T n U1 U2   ->
-      subst_type_in_type T n V1 V2   ->
-      subst_context T n (ext_cvar Gamma (U1, V1)) (ext_cvar Gamma' (U2, V2)).
-
-Hint Constructors subst_context.
 
 
 (* ################################### *)
 (** *** Coercion Relation *)
 
-Reserved Notation "Gamma '|-' t ';' T1 '~' T2" (at level 40).
+
+Reserved Notation "Gamma '|-' t ';' T1 '~~' T2" (at level 40).
     
 Inductive well_formed_coercion (Gamma : context) : cn -> ty -> ty -> Prop :=
   | C_Var : forall x T1 T2,
       well_formed_context Gamma        ->
       get_cvar Gamma x = Some (T1, T2) ->
-      Gamma |- CVar x ; T1 ~ T2
-  | C_Refl : forall T,
+      Gamma |- CVar x ; T1 ~~ T2
+  | C_Refl : forall T k,
       well_formed_context Gamma ->
-      well_formed_type Gamma T  ->
-      Gamma |- CRefl T ; T ~ T
+      well_formed_type Gamma T k ->
+      Gamma |- CRefl T ; T ~~ T
   | C_Sym : forall c T1 T2,
-      Gamma |- c ; T1 ~ T2 ->
-      Gamma |- CSym c ; T2 ~ T1
+      Gamma |- c ; T1 ~~ T2 ->
+      Gamma |- CSym c ; T2 ~~ T1
   | C_Trans : forall c1 c2 U V W,
-      Gamma |- c1 ; U ~ V ->
-      Gamma |- c2 ; V ~ W ->
-      Gamma |- CTrans c1 c2 ; U ~ W
-  | C_Arrow : forall c1 c2 U1 U2 V1 V2,
-      Gamma |- c1 ; U1 ~ V1 ->
-      Gamma |- c2 ; U2 ~ V2 ->
-      Gamma |- CArrow c1 c2 ; TArrow U1 U2 ~ TArrow V1 V2
-  | C_Forall : forall c U V,
-      ext_tvar Gamma |- c ; U ~ V ->
-      Gamma |- CTAbs c ; TUniv U ~ TUniv V
-  | C_CTCoerce : forall c1 c2 c3 U1 U2 U3 V1 V2 V3,
-      Gamma |- c1 ; U1 ~ V1 ->
-      Gamma |- c2 ; U2 ~ V2 ->
-      Gamma |- c3 ; U3 ~ V3 ->
-      Gamma |- CTCoerce c1 c2 c3 ; TCoerce U1 U2 U3 ~ TCoerce V1 V2 V3
-  | C_ALeft : forall c U1 U2 V1 V2,
-      Gamma |- c ; (TArrow U1 U2) ~ (TArrow V1 V2) ->
-      Gamma |- CNth 1 c ; U1 ~ V1
-  | C_ARight : forall c U1 U2 V1 V2,
-      Gamma |- c ; (TArrow U1 U2) ~ (TArrow V1 V2) ->
-      Gamma |- CNth 2 c ; U2 ~ V2
-  | C_CLeft11 : forall c U1 U2 S V1 V2 T,
-      Gamma |- c ; TCoerce U1 U2 S ~ TCoerce V1 V2 T ->
-      Gamma |- CNth 1 c ; U1 ~ V1 
-  | C_CLeft12 : forall c U1 U2 S V1 V2 T,
-      Gamma |- c ; TCoerce U1 U2 S ~ TCoerce V1 V2 T ->
-      Gamma |- CNth 2 c ; U2 ~ V2
-  | C_CRight : forall c U1 U2 S V1 V2 T,
-      Gamma |- c ; TCoerce U1 U2 S ~ TCoerce V1 V2 T ->
-      Gamma |- CNth 3 c ; S ~ T  
-  | C_Inst : forall c U V T,
-      Gamma |- c ; TUniv U ~ TUniv V ->
-      well_formed_type Gamma T       ->
-      Gamma |- CTApp c T ; ([0 := T] U) ~ ([0 := T] V)
+      Gamma |- c1 ; U ~~ V ->
+      Gamma |- c2 ; V ~~ W ->
+      Gamma |- CTrans c1 c2 ; U ~~ W
+  | C_App : forall c1 c2 U1 U2 V1 V2,
+      Gamma |- c1 ; U1 ~~ V1 ->
+      Gamma |- c2 ; U2 ~~ V2 ->
+      well_formed_type Gamma (TApp U1 U2) KStar ->
+      well_formed_type Gamma (TApp V1 V2) KStar ->                    
+      Gamma |- CApp c1 c2 ; TApp U1 U2 ~~ TApp V1 V2
+  | C_Forall : forall c U V k,
+      ext_tvar Gamma k |- c ; U ~~ V ->
+      well_formed_type Gamma (TUniv k U) KStar ->
+      well_formed_type Gamma (TUniv k V) KStar ->
+      Gamma |- CTAbs k c ; TUniv k U ~~ TUniv k V
+
+  | C_ALeft : forall c U1 U2 V1 V2 k1 k2,
+      well_formed_type Gamma U1 (KArrow k1 k2) ->
+      well_formed_type Gamma V1 (KArrow k1 k2) ->
+      Gamma |- c ; (TApp U1 U2) ~~ (TApp V1 V2) ->
+      Gamma |- CNth 1 c ; U1 ~~ V1
+                                          
+  | C_ARight : forall c U1 U2 V1 V2 k,
+      well_formed_type Gamma U2 k ->
+      well_formed_type Gamma V2 k ->
+      Gamma |- c ; (TApp U1 U2) ~~ (TApp V1 V2) ->
+      Gamma |- CNth 2 c ; U2 ~~ V2
+
+  | C_Inst : forall c U V T k,
+      Gamma |- c ; TUniv k U ~~ TUniv k V ->
+      well_formed_type Gamma T k      ->
+      Gamma |- CTApp c T ; ([0 := T] U) ~~ ([0 := T] V)
     
-where "Gamma '|-' c ';' T1 '~' T2" := (well_formed_coercion Gamma c T1 T2).
+where "Gamma '|-' c ';' T1 '~~' T2" := (well_formed_coercion Gamma c T1 T2).
 
 Tactic Notation "coercion_cases" tactic(first) ident(c) :=
   first;
   [ Case_aux c "C_Var"   | Case_aux c "C_Refl" 
   | Case_aux c "C_Sym"   | Case_aux c "C_Trans" 
-  | Case_aux c "C_Arrow" | Case_aux c "C_Forall"
-  | Case_aux c "C_CTCoerce"
+  | Case_aux c "C_App"   | Case_aux c "C_Forall"
   | Case_aux c "C_ALeft" | Case_aux c "C_ARight"
-  | Case_aux c "C_CLeft11" | Case_aux c "C_CLeft12"
-  | Case_aux c "C_CRight"  | Case_aux c "C_Inst" ].
+  | Case_aux c "C_Inst" ].
 
 Hint Constructors well_formed_coercion.
 
@@ -228,38 +212,42 @@ Hint Constructors well_formed_coercion.
 (** *** Typing Relation *)
 
 Reserved Notation "Gamma '|-' t '\in' T" (at level 40).
-    
+
+
+Definition tArrow (t1 : ty) (t2:ty) := TApp (TApp (TCon TArrow) t1) t2.
+Definition tCoerce k t1 t2 t3 := TApp (TApp (TApp (TCon (TEq k)) t1) t2) t3.
 Inductive has_type : context -> tm -> ty -> Prop :=
   | T_Var : forall Gamma x T,
       well_formed_context Gamma ->
       get_var Gamma x = Some T ->
       Gamma |- tvar x \in T
   | T_Abs : forall Gamma T11 T12 t12,
+      well_formed_type Gamma T11 KStar ->               
       ext_var Gamma T11 |- t12 \in T12 -> 
-      Gamma |- tabs T11 t12 \in TArrow T11 T12
+      Gamma |- tabs T11 t12 \in tArrow T11 T12
   | T_App : forall T11 T12 Gamma t1 t2,
-      Gamma |- t1 \in TArrow T11 T12 -> 
+      Gamma |- t1 \in tArrow T11 T12 -> 
       Gamma |- t2 \in T11 -> 
       Gamma |- tapp t1 t2 \in T12
-  | T_TAbs : forall Gamma t T,
-      ext_tvar Gamma |- t \in T ->
-      Gamma |- ttabs t \in (TUniv T)
-  | T_TApp : forall Gamma t1 T12 T2,
-      Gamma |- t1 \in (TUniv T12) ->
-      well_formed_type Gamma T2   ->
+  | T_TAbs : forall Gamma t T k,
+      ext_tvar Gamma k |- t \in T ->
+      Gamma |- ttabs k t \in (TUniv k T)
+  | T_TApp : forall Gamma t1 T12 T2 k,
+      Gamma |- t1 \in (TUniv k T12) ->
+      well_formed_type Gamma T2 k  ->
       well_formed_context Gamma   ->
       Gamma |- ttapp t1 T2 \in [0 := T2] T12
-  | T_CAbs : forall Gamma t T1 T2 T,
+  | T_CAbs : forall Gamma t T1 T2 T k,
       ext_cvar Gamma (T1, T2) |- t \in T ->
-      well_formed_type Gamma T1 ->
-      well_formed_type Gamma T2 ->
-      Gamma |- tcabs T1 T2 t \in TCoerce T1 T2 T
-  | T_CApp : forall Gamma U1 U2 T t c,
-      Gamma |- t \in (TCoerce U1 U2 T) ->
-      Gamma |- c ; U1 ~ U2             ->
+      well_formed_type Gamma T1 k ->
+      well_formed_type Gamma T2 k ->
+      Gamma |- tcabs T1 T2 t \in tCoerce k T1 T2 T
+  | T_CApp : forall Gamma U1 U2 T t c k,
+      Gamma |- t \in (tCoerce k U1 U2 T) ->
+      Gamma |- c ; U1 ~~ U2             ->
       Gamma |- tcapp t c \in T
   | T_Coerce : forall Gamma t c T1 T2,
-      Gamma |- c ; T1 ~ T2 ->
+      Gamma |- c ; T1 ~~ T2 ->
       Gamma |- t \in T1    ->
       Gamma |- tcoerce t c \in T2
 
@@ -274,5 +262,63 @@ Tactic Notation "has_type_cases" tactic(first) ident(c) :=
   | Case_aux c "T_CApp" | Case_aux c "T_Coerce" ].
 
 Hint Constructors has_type.
+
+
+(* ####################################################### *)
+(** *** Uniqueness: our judgements are syntax directed.    *)
+
+Lemma kinds_unique :
+  forall Gamma U k1, well_formed_type Gamma U k1 ->
+    forall k2, well_formed_type Gamma U k2 -> k1 = k2.
+Proof.
+  induction 1; intros k2 H2; inversion H2.
+  rewrite H in H1. inversion H1. auto.
+  rewrite H in H1. inversion H1. auto.
+  apply IHwell_formed_type1 in H4.
+  apply IHwell_formed_type2 in H6. subst.
+  inversion H4. auto.
+  auto.
+Qed.
+
+
+Lemma props_unique :
+  forall Gamma cn U1 V1,
+    Gamma |- cn ; U1 ~~ V1 ->
+      forall U2 V2, Gamma |- cn ; U2 ~~ V2 ->
+                                  U1 = U2 /\ V1 = V2.
+Proof.
+  induction 1; intros U1' U2' K2; inversion K2; subst.
+  - rewrite H0 in H3. inversion H3. auto.
+  - auto.
+  - destruct (IHwell_formed_coercion _ _ H1). subst. auto.
+  - destruct (IHwell_formed_coercion1 _ _ H3).
+    destruct (IHwell_formed_coercion2 _ _ H6). subst. auto.
+  - destruct (IHwell_formed_coercion1 _ _ H5).
+    destruct (IHwell_formed_coercion2 _ _ H6). subst. auto.
+  - destruct (IHwell_formed_coercion _ _ H4). subst. auto.
+  - destruct (IHwell_formed_coercion _ _ H5).
+    inversion H2. inversion H6. subst. auto.
+  - destruct (IHwell_formed_coercion _ _ H5).
+    inversion H2. inversion H6. subst. auto.
+  - destruct (IHwell_formed_coercion _ _ H3).
+    inversion H1. inversion H2. subst. auto.
+Qed.
+
+Lemma types_unique:
+  forall Gamma tm T1, (Gamma |- tm \in T1) ->
+                      forall T2,( Gamma |- tm \in T2) -> T1 = T2.
+Proof.
+  induction 1; intros T' H2; inversion H2; subst.
+  - rewrite H0 in H5. inversion H5. trivial.
+  - rewrite IHhas_type with T1; trivial.
+  - pose (J:= IHhas_type1 _ H5). inversion J. trivial.
+  - rewrite IHhas_type with T0; trivial.
+  - pose (J:= IHhas_type _ H5). inversion J. trivial.
+  - rewrite IHhas_type with T4; trivial.
+    rewrite kinds_unique with Gamma T1 k k0; trivial.
+  - pose (J:= IHhas_type _ H5). inversion J. trivial.
+  - destruct (props_unique _ _ _ _ H _ _ H5). trivial.
+Qed.    
+
 
 End TYPING.
